coq_stuff/groups.v
@@ -1,0 +1,63 @@
+
+(* The set of the group. *)
+Section Group.
+Variable G : Set.
+
+(* The binary operator. *)
+Variable f : G -> G -> G.
+
+(* The group identity. *)
+Variable e : G.
+
+(* The inverse operator. *)
+Variable i : G -> G.
+
+(* For readability, we use infix <+> to stand for the binary operator. *)
+Infix "<+>" := f (at level 50, left associativity).
+
+(* The operator [f] is associative. *)
+Variable assoc : forall a b c, a <+> b <+> c = a <+> (b <+> c).
+
+(* [e] is the right-identity for all elements [a] *)
+Variable id_r : forall a, a <+> e = a.
+
+Variable id_l : forall a, e <+> a = a.
+(* [i a] is the right-inverse of [a]. *)
+Variable inv_r : forall a, a <+> i a = e.
+
+Variable inv_l : forall a, i a <+> a = e.
+Lemma mult_both_sides : forall a b c : G, a = b -> c <+> a = c <+> b.
+Proof.
+  intros. rewrite H. reflexivity.
+Qed.
+
+Lemma mult_both_sides' : forall a b c : G, a = b -> a <+> c = b <+> c.
+Proof.
+  intros. rewrite H. reflexivity.
+Qed.
+Theorem cancel_left : forall a b c : G, a <+> b = a <+> c -> b = c.
+Proof.
+  intros. apply mult_both_sides with (c := i a) in H.
+  rewrite <- assoc in H. rewrite <- assoc in H.
+  rewrite inv_l in H. rewrite id_l in H. rewrite id_l in H.
+  apply H.
+Qed.
+Theorem cancel_right : forall a b c : G, b <+> a = c <+> a -> b = c.
+Proof.
+  intros. apply mult_both_sides' with (c := i a) in H.
+  rewrite assoc in H. rewrite assoc in H.
+  rewrite inv_r in H. rewrite id_r in H. rewrite id_r in H.
+  apply H.
+Qed.
+
+Theorem id_unique : forall e1 : G, (forall d : G, e1 <+> d = d ->
+  e1 = e).
+Proof.
+  intros. apply mult_both_sides' with (c := i d) in H.
+  rewrite assoc in H. rewrite inv_r in H. rewrite id_r in H.
+  apply H.
+Qed.
+
+End Group.
+ 
+
